---
title: Homework 4
author: Christopher Achenbach
fontsize: 12pt
---

Problems from 2.6
================================================================================

7.
\begin{displaymath}
\begin{array}{|c|c|c|c|c|c|c|}
p & q & \neg q & p \land \neg q & q \land \neg q & (p \land \neg q) \to (q \land \neg q) & p \to q \\ \hline
1 & 1 & 0 & 0 & 0 & 1 & 1 \\
1 & 0 & 1 & 1 & 0 & 0 & 0 \\
0 & 1 & 0 & 0 & 0 & 1 & 1 \\
0 & 0 & 1 & 0 & 0 & 1 & 1
\end{array}
\end{displaymath}
Therefore, $(p \land \neg q) \to (q \land \neg q)  \ = \  p \to q$.

8.
\begin{displaymath}
\begin{array}{|c|c|c|c|c|c|c|c|}
p & q & \neg p & \neg q & p \to \neg q & \neg q \to p & (p \to \neg q) \land (\neg q \to p) & \neg p \leftrightarrow q \\ \hline
1 & 1 & 0 & 0 & 0 & 1 & 0 & 0 \\
1 & 0 & 0 & 1 & 1 & 1 & 1 & 1 \\
0 & 1 & 1 & 0 & 1 & 1 & 1 & 1 \\
0 & 0 & 1 & 1 & 1 & 0 & 0 & 0
\end{array}
\end{displaymath}
Therefore, $\neg p \leftrightarrow q  \ = \ (p \to \neg q) \land (\neg q \to p)$.

<!--  -->
\pagebreak

10.
\begin{displaymath}
\begin{array}{|c|c|c|c|c|c|c|c|c|c|c|c|c|}
p & q & r & \neg q & \neg r & p \to q & p \land \neg q & (p \land \neg q) \land \neg r & \neg ((p \land \neg q) \land \neg r) & (p \to q) \lor r \\ \hline
1 & 1 & 1 & 0 & 0 & 1 & 0 & 0 & 1 & 1 \\
1 & 1 & 0 & 0 & 1 & 1 & 0 & 0 & 1 & 1 \\
1 & 0 & 1 & 1 & 0 & 0 & 1 & 0 & 1 & 1 \\
0 & 0 & 0 & 1 & 1 & 1 & 0 & 0 & 1 & 1 \\
0 & 1 & 1 & 0 & 0 & 1 & 0 & 0 & 1 & 1 \\
0 & 1 & 0 & 0 & 1 & 1 & 0 & 0 & 1 & 1
\end{array}
\end{displaymath}
Therefore, $\neg ((p \land \neg q) \land \neg r) \ = \ (p \to q) \lor r$.
Yes, they are logically equivalent.

11.
\begin{displaymath}
\begin{array}{|c|c|c|c|c|c|c|c|}
p & q & \neg p & p \to q & q \to p & (\neg p) \land (p \to q) & \neg (q \to p) \\ \hline
1 & 1 & 0 & 1 & 1 & 0 & 0 \\
1 & 0 & 0 & 0 & 1 & 0 & 0 \\
0 & 1 & 1 & 1 & 0 & 1 & 1 \\
0 & 0 & 1 & 1 & 1 & 1 & 0
\end{array}
\end{displaymath} 
Therefore, $(\neg p) \land (p \to q) \ \not = \ \neg (q \to p)$.
No, they are not logically equivalent. In the case where both $p$ is false and $q$ is false, the two statements are not the same.

12.
\begin{displaymath}
\begin{array}{|c|c|c|c|c|c|c|c|}
p & q & \neg q & p \to q & \neg (p \to q) & p \land \neg q \\ \hline
1 & 1 & 0 & 1 & 0 & 0 \\
1 & 0 & 1 & 0 & 1 & 1 \\
0 & 1 & 0 & 1 & 0 & 0 \\
0 & 0 & 1 & 1 & 0 & 0
\end{array}
\end{displaymath} 
Therefore, $\neg (p \to q) \ = \ p \land \neg q$. Yes, they are logically equivalent.







Problems from 2.7
================================================================================

1.

<!--  -->

3.

4.

5.

<!--  -->

7.