---
title: Homework 8
author: Christopher Achenbach
fontsize: 12pt
---

# Problem 1

**Proposition**. For $n \in \mathbb{Z}$, If $n^2$ is even, then $n$ is even.

*Proof*. (Contrapositive). Suppose $n$ is not even.\
Thus, $n$ is odd, and can be expressed by the 
equation $n = 2x+1$ for some integer $x$.
Squaring $n$ and substituting, we find that
$$
    \begin{aligned}
        n^2 &= (2x+1)^2 \\
        &= 4x^2 + 4x + 1 \\
        &= 2(2x^2 + 2x) + 1
    \end{aligned}
$$
Let $z$ be an integer such that $z = 2x^2 + 2x$, which allows us to rewrite the equation above as
$$
    n^2 = 2z + 1
$$
which reveals that $n^2$ is odd.\
Therefore, $n^2$ is not even.
\hfill $\blacksquare$ 

\newpage


# Problem 3 

**Proposition**. For $a,b \in \mathbb{Z}$, If $a^2(b^2-2b)$ is odd, then $a$ and $b$ are odd.

*Proof*. (Contrapositive). Suppose  $a$ is not odd or $b$ is not odd.\
Let $x$, $y$ and $z$ be integers.

**Case 1**. $a$ is not odd, $b$ is not odd.\
We can represent $a$ and $b$ using the equations $a=2x$ and $b=2y$.\
Using these definitions of $a$ and $b$, we can write the equality,
$$
    \begin{aligned}
        a^2(b^2-2b) &= (2x)^2 \big( (2y)^2 - 2(2y) \big) \\
        &= 4x^2 (4y^2 - 4y) \\
        &= 2(8x^2y^2 - 8x^2y)
    \end{aligned}
$$
Let integer $z = 8x^2y^2 - 8x^2y$, and substitute into the equality above,
$$
    a^2(b^2-2b) = 2z
$$
Therefore, $a^2(b^2-2b)$ is not odd.

**Case 2**. $a$ is not odd, $b$ is odd.\
We can represent $a$ and $b$ using the equations $a = 2x$, and $b = 2y+1$. 
Using these definitions of $a$ and $b$, we can write the equality,
$$
    \begin{aligned}
        a^2(b^2-2b) &= (2x)^2 \big( (2y+1)^2 - 2(2y+1) \big)\\
        &= 4x^2 (4y^2)\\
        &= 2(8x^2y^2)
    \end{aligned}
$$
Let integer $z = 8x^2y^2$ and substitute into the equality above,
$$
    a^2(b^2-2b) = 2z
$$
Therefore, $a^2(b^2-2b)$ is not odd.

**Case 3**. $a$ is odd, $b$ is not odd.\
We can represent $a$ and $b$ using the equations $a = 2x+1$, and $b = 2y$. 
Using these definitions of $a$ and $b$, we can write the equality,
$$
    \begin{aligned}
        a^2(b^2-2b) &= (2x+1)^2 \big( (2y)^2 - 2(2y) \big)\\
        &= (4x^2 + 4x +1)(4y^2 - 4y) \\
        &= 2 \cdot (4x^2 + 4x +1)(2y^2 - 2y)
    \end{aligned}
$$
Let integer $z = (4x^2 + 4x +1)(2y^2 - 2y)$ and substitute into the equality above,
$$
    a^2(b^2-2b) = 2z
$$
Therefore, $a^2(b^2-2b)$ is not odd.
\hfill $\blacksquare$ 




\newpage

# Problem 7

**Proposition**. For $a,b \in \mathbb{Z}$, If both $ab$ and $a+b$ are even, then both $a$ and $b$ are even.

*Proof*. (Contrapositive). Suppose either $a$ is not even, or $b$ is not even.\
For each of these cases, it will be sufficient to prove that either $ab$ is not even, or $a+b$ is not even.

**Case 1**. $a$ is not even, $b$ is even.\
Let $a=2x+1$ and $b=2y$ for some $x,y \in \mathbb{Z}$. So,
$$
    \begin{aligned}
        a + b &= 2x+1+2y \\
        &= 2(x+y) + 1
    \end{aligned}
$$
Let some integer $z = x+y$. Thus, $a+b = 2z+1$. Therefore, $a+b$ is not even.

**Case 2**. $a$ is even, $b$ is not even.\
This case is actually identical to Case 1, because we can let $a=2y$ and $b=2x+1$ for some $x,y \in \mathbb{Z}$, and due to the Commutative Law of Addition,
$$
    a + b = b +a
$$
Hence, we can apply Case 1. Therefore, $a+b$ is not even.

**Case 3**. $a$ is not even, $b$ is not even.\
Let $a=2x+1$ and $b=2y+1$ for some $x,y \in \mathbb{Z}$. So,
$$
    \begin{aligned}
        ab &= (2x+1)(2y+1) \\
        &= 4xy + 2x + 2y + 1 \\
        &= 2(2xy+x+y) +1\\
    \end{aligned}
$$
Let some integer $z = 2xy+x+y$. Thus, $ab = 2z+1$. Therefore, $ab$ is not even.

Therefore, in summary of all cases, either $ab$ or $a+b$ is not even.
\hfill $\blacksquare$ 



\newpage

# Problem 12


**Proposition**. For $a \in \mathbb{Z}$, If $a^2 \nmid 4$, then $a$ is odd.

*Proof*. (Contrapositive). Suppose $a$ is not odd.\
Let $a=2x$ for some $x\in\mathbb{Z}$. So,
$$
\begin{aligned}
    a^2 &= (2x)^2\\
    &= 4(x^2)
\end{aligned}
$$
Let some integer $z = x^2$. Thus $a^2 = 4z$. Therefore $a^2$ is divisible by 4.
\hfill $\blacksquare$ 
